---
title: "Random Number Generation for Generalized Poisson Distribution"
author: >
  [Eduardo E. Ribeiro Jr](https://jreduardo.github.io/) &
  [Walmes Marques Zeviani](http://www.leg.ufpr.br/~walmes)
vignette: >
  %\VignetteIndexEntry{Random Number Generation for Generalized Poisson Distribution}
  %\VignetteEngine{knitr::rmarkdown}
  %\VignetteEncoding{UTF-8}
---

For some discrete random variables, is possible calculate probabilities
using a recursive formula. Bionomial and Poisson random variables have
these property. Lets check if the same apply for the Generalized Poisson
(GP) distribution.

$$
\begin{align*}
\Pr(X = x) &= \Pr(X = x - 1) \times h(x)\\
h(x) &= \frac{\Pr(X = x)}{\Pr(X = x - 1)}\\
 &= \frac{
  \left(\frac{\lambda}{1+\alpha\lambda}\right)^{y}
  (1 + \alpha y)^{y - 1}
  \exp\left\{-\lambda\frac{1+\alpha y}{1+\alpha\lambda}\right\}
  (y!)^{-1}}{
  \left(\frac{\lambda}{1+\alpha\lambda}\right)^{y - 1}
  (1 + \alpha (y - 1))^{y - 2}
  \exp\left\{-\lambda\frac{1+\alpha (y - 1)}{1+\alpha\lambda}\right\}
  ((y - 1)!)^{-1}}\\
 &= \frac{\left(\frac{\lambda}{1+\alpha\lambda}\right)^{y}}{
          \left(\frac{\lambda}{1+\alpha\lambda}\right)^{y-1}} \times
    \frac{(1 + \alpha y)^{y - 1}}{
          (1 + \alpha (y - 1))^{y - 2}} \times
    \frac{\exp\left\{-\lambda\frac{1+\alpha y}{
          1+\alpha\lambda}\right\}}{
          \exp\left\{-\lambda\frac{1+\alpha (y - 1)}{
          1+\alpha\lambda}\right\}} \times
    \frac{(y!)^{-1}}{((y - 1)!)^{-1}}\\
 &= \left(\frac{\lambda}{1+\alpha\lambda}\right) \times
    (1 + \alpha y)^{y - 1}(1 + \alpha (y - 1))^{2 - y} \times
    \exp\left\{-\frac{\alpha\lambda}{1+\alpha\lambda}\right\} \times
    y^{-1}
\end{align*}
$$

These property is valid for GP distribution. Note that is recursive
formula is only valid for values of $x > 1$. For $\Pr(X=0)$ and
$\Pr(X=1)$ should be used the probability function.

$$
\begin{align*}
\Pr(X = 0) &=
  \left(\frac{\lambda}{1+\alpha\lambda}\right)^{0}
  (1 + \alpha 0)^{0 - 1}
  \exp\left\{-\lambda\frac{1+\alpha 0}{1+\alpha\lambda}\right\} =
  \exp\left\{-\frac{\lambda}{1+\alpha\lambda}\right\} \\
\Pr(X = 1) &= \left(\frac{\lambda}{1+\alpha\lambda}\right)^{1}
  (1 + \alpha 1)^{1 - 1}
  \exp\left\{-\lambda\frac{1+\alpha 1}{1+\alpha\lambda}\right\} =
  \left(\frac{\lambda}{1+\alpha\lambda}\right)
  \exp\left\{-\lambda\frac{1+\alpha}{1+\alpha\lambda}\right\}
\end{align*}
$$
